src/tls/test/TestRecord.fst
@@ -14,7 +14,7 @@ private let mk_id pv aeAlg =
   let kdf = match pv with
   | TLS_1p0 -> PRF_SSL3_concat
   | TLS_1p1 -> PRF_TLS_1p01 kdf_label
-  | TLS_1p2 -> PRF_TLS_1p2 kdf_label (HMAC CoreCrypto.SHA256) in
+  | TLS_1p2 -> PRF_TLS_1p2 kdf_label (HMAC Hashing.Spec.SHA256) in
   let gx = CommonDH.keygen (CommonDH.ECDH CoreCrypto.ECC_P256) in
   let g = CommonDH.key_params gx in
   let gy, gxy = CommonDH.dh_responder gx in
@@ -22,7 +22,7 @@ private let mk_id pv aeAlg =
   ID12 pv msid kdf aeAlg er er Client
 
 private let mk_id13 aeAlg =
-  let hash_alg = CoreCrypto.SHA256 in
+  let hash_alg = Hashing.Spec.SHA256 in
   let gx = CommonDH.keygen (CommonDH.ECDH CoreCrypto.ECC_P256) in
   let gy,_ = CommonDH.dh_responder gx in
   let initiator = CommonDH.share_of_key gx in
@@ -180,17 +180,17 @@ private let test_cbc pv aeAlg seqn key iv plain cipher macKey =
 
 val main : unit -> ML unit
 let main () =
-  test_stream (AEAD CoreCrypto.AES_128_GCM CoreCrypto.SHA256)
+  test_stream (AEAD CoreCrypto.AES_128_GCM Hashing.Spec.SHA256)
     "152300c2dc44c8f695d4fb1471791659"
     "b56bf932b56bf932ffffffff"
     "474554202f20485454502f312e310d0a486f73743a20756e646566696e65640d0a0d0a"
     "bd324f59c8ff0eb7fcdc519e0fd84203fbc1efcdca0c7f3160d8856cebe3e340fedc8ea409093a847e9b8d5863bf5a4899d453e11447de6f0068341625120b0d9b03b57595a74fb89d7a6ae6bdb7b3ac";
-  test_aead TLS_1p2 (AEAD CoreCrypto.AES_128_GCM CoreCrypto.SHA256)
+  test_aead TLS_1p2 (AEAD CoreCrypto.AES_128_GCM Hashing.Spec.SHA256)
     "152300c2dc44c8f695d4fb1471791659"
     "b56bf932"
     "474554202f20485454502f312e310d0a486f73743a20756e646566696e65640d0a0d0a"
     "0000000000000000ed3ca96c8bd2fbb376c2dc417f3ec249e8ab550dab1c421293f0e642a0c152b43a546aa26bbe62e8651214d28ab90e70217b3d";
-  test_cbc TLS_1p2 (MtE (Block CoreCrypto.AES_128_CBC) CoreCrypto.SHA1) 1
+  test_cbc TLS_1p2 (MtE (Block CoreCrypto.AES_128_CBC) Hashing.Spec.SHA1) 1
     "e77f6871e1697b2286416f973aee9ff6"
     "00000000000000000000000000000000"
     "474554202f20485454502f312e310d0a486f73743a20756e646566696e65640d0a0d0a"
